prove bedrock2 x25519 wrappers

src/Bedrock/End2End/X25519/MontgomeryLadder.v
@@ -9,44 +9,26 @@ Require Import compiler.Symbols.
 Require Import compiler.MMIO.
 Require Import coqutil.Word.Bitwidth32.
 Require Import Crypto.Arithmetic.PrimeFieldTheorems.
-Require Import Crypto.Bedrock.End2End.X25519.Field25519.
 Require Import Crypto.Bedrock.Field.Interface.Compilation2.
 Require Import Crypto.Bedrock.Field.Synthesis.New.UnsaturatedSolinas.
 Require Import Crypto.Bedrock.Group.AdditionChains.
 Require Import Crypto.Bedrock.Group.ScalarMult.LadderStep.
 Require Import Crypto.Bedrock.Group.ScalarMult.CSwap.
 Require Import Crypto.Bedrock.Group.ScalarMult.MontgomeryLadder.
+Require Import Crypto.Bedrock.End2End.X25519.Field25519.
 Local Open Scope string_scope.
 Import ListNotations.
 
 
-Derive ladderstep SuchThat
-       (ladderstep = ladderstep_body
-                       (BW:=BW32)
-                       (field_parameters:=field_parameters)
-                       (field_representaton:=field_representation n s c))
-       As ladderstep_defn.
+Local Instance frep25519 : Field.FieldRepresentation(field_parameters:=field_parameters) := field_representation n Field25519.s c.
+Derive ladderstep SuchThat (ladderstep = ladderstep_body) As ladderstep_defn.
 Proof. vm_compute. subst; exact eq_refl. Qed.
 
-Derive montladder SuchThat
-       (montladder
-        = montladder_body
-            (BW:=BW32)
-            (Z.to_nat (Z.log2 Curve25519.order))
-            (field_parameters:=field_parameters)
-            (field_representaton:=field_representation n s c))
+Derive montladder SuchThat (montladder = montladder_body (Z.to_nat (Z.log2 Curve25519.order)))
        As montladder_defn.
 Proof. vm_compute. subst; exact eq_refl. Qed.
 
-Import String.
 Require Import bedrock2.NotationsCustomEntry.
-Require Import bedrock2Examples.LAN9250.
-Require Import bedrock2Examples.lightbulb.
-Require Import bedrock2Examples.chacha20.
-Require Import bedrock2Examples.memequal.
-Require Import bedrock2Examples.memswap.
-Require Import bedrock2Examples.memconst.
-Require Import Rupicola.Examples.Net.IPChecksum.IPChecksum.
 
 Definition x25519 : func := ("x25519", (["out"; "sk"; "pk"], [], bedrock_func_body:(
   stackalloc 40 as U;
@@ -64,15 +46,141 @@ Definition x25519_base : func := ("x25519_base", (["out"; "sk"], [], bedrock_fun
   fe25519_to_bytes(out, OUT)
 ))).
 
+Import LittleEndianList.
+Local Coercion F.to_Z : F >-> Z.
+Require Import bedrock2.WeakestPrecondition bedrock2.Semantics bedrock2.ProgramLogic.
+Require Import bedrock2.BasicC32Semantics bedrock2.Syntax bedrock2.Map.SeparationLogic.
+Require Import coqutil.Map.OfListWord Coq.Init.Byte coqutil.Byte.
+Import ProgramLogic.Coercions.
+Local Notation "m =* P" := ((P%sep) m) (at level 70, only parsing) (* experiment*).
+Local Notation "xs $@ a" := (Array.array ptsto (word.of_Z 1) a xs) (at level 10, format "xs $@ a").
+Definition x25519_gallina := montladder_gallina (Field.M_pos(FieldParameters:=field_parameters)) Field.a24 (Z.to_nat (Z.log2 (Z.pos order))).
+Global Instance spec_of_x25519 : spec_of x25519 :=
+  fnspec! "x25519" out sk pk / (o s p : list Byte.byte) (R : mem -> Prop),
+  { requires t m := m =* s$@sk * p$@pk * o$@out * R /\
+      length s = 32%nat /\ length p = 32%nat /\ length o = 32%nat /\ byte.unsigned (nth 31 p x00) <= 0x7f;
+    ensures t' m := t=t' /\ m=* s$@sk ⋆ p$@pk ⋆ R ⋆
+      (le_split 32 (x25519_gallina (le_combine s) (Field.feval_bytes p)))$@out }.
+
+Local Instance spec_of_fe25519_from_word : spec_of "fe25519_from_word" := Field.spec_of_from_word.
+Local Instance spec_of_fe25519_from_bytes : spec_of "fe25519_from_bytes" := Field.spec_of_from_bytes.
+Local Instance spec_of_fe25519_to_bytes : spec_of "fe25519_to_bytes" := Field.spec_of_to_bytes.
+Local Instance spec_of_montladder : spec_of "montladder" := spec_of_montladder(Z.to_nat (Z.log2 Curve25519.order)).
+Lemma x25519_ok : program_logic_goal_for_function! x25519.
+Proof.
+  repeat straightline.
+  seprewrite_in (@Bignum.Bignum_of_bytes _ _ _ _ _ _ 10 a) H2. { transitivity 40%nat; trivial. }
+
+  straightline_call; ssplit.
+  { eexists. ecancel_assumption. }
+  { unfold Field.FElem.
+    use_sep_assumption. cancel. cancel_seps_at_indices 0%nat 0%nat; cbn; trivial. eapply RelationClasses.reflexivity. }
+  { unfold Field.bytes_in_bounds, frep25519, field_representation, Signature.field_representation, Representation.frep.
+    match goal with |- ?P ?x ?z => let y := eval cbv in x in change (P y z) end; cbn.
+    repeat (destruct p as [|? p]; try (cbn in *;discriminate); []).
+    cbn; cbn [nth] in *.
+    cbv [COperationSpecifications.list_Z_bounded_by FoldBool.fold_andb_map map seq]; cbn.
+    pose proof byte.unsigned_range as HH. setoid_rewrite <-Le.Z.le_sub_1_iff in HH. cbn in HH.
+    setoid_rewrite Zle_is_le_bool in HH. setoid_rewrite <-Bool.andb_true_iff in HH.
+    rewrite 31HH; cbn.
+    eapply Bool.andb_true_iff; split; trivial.
+    eapply Bool.andb_true_iff; split; eapply Zle_is_le_bool; trivial.
+    eapply byte.unsigned_range. }
+  repeat straightline.
+
+  seprewrite_in (@Bignum.Bignum_of_bytes _ _ _ _ _ _ 10 a2) H15. { transitivity 40%nat; trivial. }
+
+  straightline_call; ssplit.
+  3: { unfold FElem, Field.FElem in *; extract_ex1_and_emp_in_goal; ssplit.
+       { use_sep_assumption. cancel; repeat ecancel_step.
+       cancel_seps_at_indices 0%nat 0%nat; trivial. cbn; reflexivity. }
+    all : eauto.
+    { instantiate (1:=None). exact I. } }
+  { reflexivity. }
+  { rewrite H3. vm_compute. inversion 1. }
+  repeat straightline.
+
+  unfold FElem in H22. extract_ex1_and_emp_in H22.
+  straightline_call; ssplit.
+  { ecancel_assumption. }
+  { transitivity 32%nat; auto. }
+  { eexists. ecancel_assumption. }
+  { intuition idtac. }
+  repeat straightline_cleanup.
+  repeat straightline.
+
+  cbv [Field.FElem] in *.
+  seprewrite_in @Bignum.Bignum_to_bytes H25.
+  seprewrite_in @Bignum.Bignum_to_bytes H25.
+  extract_ex1_and_emp_in H25.
+
+  repeat straightline; intuition eauto.
+  rewrite H29 in *. cbv [x25519_gallina].
+  use_sep_assumption; cancel. eapply RelationClasses.reflexivity.
+Qed.
+
+Global Instance spec_of_x25519_base : spec_of x25519_base :=
+  fnspec! "x25519_base" out sk / (o s : list Byte.byte) (R : mem -> Prop),
+  { requires t m := m =* s$@sk * o$@out * R /\
+      length s = 32%nat /\ length o = 32%nat;
+    ensures t' m := t=t' /\ m=* s$@sk ⋆ R ⋆
+      (le_split 32 (x25519_gallina (le_combine s) (F.of_Z _ 9)))$@out }.
+
+Lemma x25519_base_ok : program_logic_goal_for_function! x25519_base.
+Proof.
+  repeat straightline.
+  seprewrite_in (@Bignum.Bignum_of_bytes _ _ _ _ _ _ 10 a) H2. { transitivity 40%nat; trivial. }
+  straightline_call; ssplit.
+  { cbv [Field.FElem]. cbn. cbv [n]. ecancel_assumption. }
+  repeat straightline.
+
+  seprewrite_in (@Bignum.Bignum_of_bytes _ _ _ _ _ _ 10 a2) H13. { transitivity 40%nat; trivial. }
+
+  straightline_call; ssplit.
+  3: { unfold FElem, Field.FElem in *; extract_ex1_and_emp_in_goal; ssplit.
+       { use_sep_assumption. cancel; repeat ecancel_step.
+       cancel_seps_at_indices 0%nat 0%nat; trivial. cbn; reflexivity. }
+    all : eauto.
+    { instantiate (1:=None). exact I. } }
+  { reflexivity. }
+  { rewrite H3. vm_compute. inversion 1. }
+  repeat straightline.
+
+  unfold FElem in H20. extract_ex1_and_emp_in H20.
+  straightline_call; ssplit.
+  { ecancel_assumption. }
+  { transitivity 32%nat; auto. }
+  { eexists. ecancel_assumption. }
+  { intuition idtac. }
+  repeat straightline_cleanup.
+  repeat straightline.
+
+  cbv [Field.FElem] in *.
+  seprewrite_in @Bignum.Bignum_to_bytes H23.
+  seprewrite_in @Bignum.Bignum_to_bytes H23.
+  extract_ex1_and_emp_in H23.
+
+  repeat straightline; intuition eauto.
+  rewrite H27 in *. cbv [x25519_gallina].
+  use_sep_assumption; cancel. eapply RelationClasses.reflexivity.
+Qed.
+
+Require Import bedrock2Examples.LAN9250.
+Require Import bedrock2Examples.lightbulb.
+Require Import bedrock2Examples.chacha20.
+Require Import bedrock2Examples.memequal.
+Require Import bedrock2Examples.memswap.
+Require Import bedrock2Examples.memconst.
+Require Import Rupicola.Examples.Net.IPChecksum.IPChecksum.
+
+Import Syntax.Coercions.
+
 Definition is_udp : func := ("is_udp", (["buf"], ["r"], bedrock_func_body:(
   ethertype = (((load1(buf + $12))&$0xff) << $8) | ((load1(buf + $13))&$0xff);
   require ($(1536 - 1) < ethertype) else { r = $0 };
   protocol = (load1(buf+$23))&$0xff;
   r = (protocol == $0x11)
 ))).
-
-Import Syntax.Coercions.
-Local Coercion Z.of_nat : nat >-> Z.
 
 Import Coq.Init.Byte.
 Definition garageowner : list byte :=
@@ -95,41 +203,43 @@ Definition loop : func := ("loop", ([], [], bedrock_func_body:(
   st=$st; pk=$pk; buf=$buf;
   unpack! l, err = recvEthernet(buf);
   require !err;
-  if $(14+20+8 +32 +2+4) == l {
+  if $(14+20+8 +32 +2+4) == l { (* getpk *)
     unpack! t = is_udp(buf);
     require t;
-    chacha20_block(st, st, (*nonce*)pk, $0); (* NOTE: another impl? *)
-    x25519_base(buf+$42, st+$32);
 
     memswap(buf, buf+$6, $6); (* ethernet address *)
     memswap(buf+$(14+12), buf+$(14+16), $4); (* IP address *)
     memswap(buf+$(14+20+0), buf+$(14+20+2), $2); (* UDP port *)
     store1(buf+$(14+2), $0); (* ip length *)
     store1(buf+$(14+3), $(20+ 8+ 32+2)); (* ip length *)
+    store1(buf+$(14+10), $0); (* preliminary ip checksum *)
+    store1(buf+$(14+11), $0); (* preliminary ip checksum *)
+
+    unpack! chk = ip_checksum(buf+$14, $20);
+    store1(buf+$(14+11), chk>>$8);
+    store1(buf+$(14+10), chk);
+
     store1(buf+$(14+20+4), $0); (* udp length *)
     store1(buf+$(14+20+5), $(8+ 32+2)); (* udp length *)
     store1(buf+$(14+20+6), $0); (* udp checksum *)
     store1(buf+$(14+20+7), $0); (* udp checksum *)
 
-    store1(buf+$(14+10), $0); (* preliminary ip checksum *)
-    store1(buf+$(14+11), $0); (* preliminary ip checksum *)
-    unpack! chk = ip_checksum(buf+$14, $20);
-    store1(buf+$(14+11), chk>>$8);
-    store1(buf+$(14+10), chk);
-
-    lan9250_tx(buf, $(14+20+8+32+2));
-    x25519(st+$32, st+$32, pk)
-  } else if $(14+20+8 +16 +2+4) == l {
+    x25519_base(buf+$42, st+$32);
+    lan9250_tx(buf, $(14+20+8+32+2))
+  } else if $(14+20+8 +16 +2+4) == l { (* operate *)
     unpack! t = is_udp(buf);
     require t;
-    unpack! set0 = memequal(st+$32, buf+$(14+20+8), $16);
-    unpack! set1 = memequal(st+$(32+16), buf+$(14+20+8), $16);
+
+    stackalloc 32 as tmp;
+    x25519(tmp, st+$32, pk);
+    unpack! set0 = memequal(tmp, buf+$(14+20+8), $16);
+    unpack! set1 = memequal(tmp+$16, buf+$(14+20+8), $16);
 
     io! mmio_val = MMIOREAD($0x1001200c);
     mmio_val = mmio_val & coq:(Z.clearbit (Z.clearbit (2^32-1) 11) 12);
     output! MMIOWRITE($0x1001200c, mmio_val | (set1<<$1 | set0) << $11);
 
-    if (set0|set1) {
+    if (set0|set1) { (* rekey *)
         chacha20_block(st, st, (*nonce*)pk, $0) (* NOTE: another impl? *)
     }
   }
